%! TeX root = zettel.tex
\documentclass[class=article, crop=false]{standalone}
\usepackage[subpreambles=true]{standalone}
\input{../standalone_preamble.tex}

\begin{document}
\begin{zettel}{Kettenregel}
\begin{flashcard}[pvkg3ady]{Kettenregel}
	\begin{theorem}[Kettenregel totales Differenzial]
		$f$ diffbar an $a \in  U$ , $g$ diffbar an $ f (a) \in  U' \implies g \circ f $ diffbar an $a \in  U$.
		\[
			D_a (g \circ f) = D_{f(a)} g \circ  D_a f
		.\]
	\end{theorem}
\end{flashcard}
\end{zettel}
\end{document}

