%! TeX root = zettel.tex
\documentclass[class=article, crop=false]{standalone}
\usepackage[subpreambles=true]{standalone}
\input{../standalone_preamble.tex}

\begin{document}
\begin{zettel}{Mittelwerts"atze}
\begin{flashcard}[nxg5qj0i]{Mittelwertsatz I}
	\begin{theorem}[Mittelwertsatz I]
		Sei $\R^n \supset  U \stackrel{f}{\to} \R $ differenzierbar, $a, b \in  U$ , sodass $\gamma(t) = a + t (b-a)$ liegt in $U$ und $t \in [0,1]$ sodass gilt
		\[
			\left(D_{\gamma(t_0)}\right) (b - a ) = f(b) - f(a)
		.\]
	\end{theorem}
\end{flashcard}

\begin{corollary}
	Sei $f$ wie oben, $\R^n \supset  U$ offen und zusammenh"angend, $D_a f = 0 \quad \forall a \in  U$ . Dann ist $f$ konstant.
\end{corollary}

\begin{flashcard}[ox7gzhr6]{Mittelwertsatz II}
	\begin{theorem}[Mittelwertsatz II]
		$V = K^n, \quad f \in  C^1 ( B_r(a)), \quad a \in  V$. Dann gibt es stetige Funktionen $ q_1,\dots,q_n \in  C ( B_r(a))$ , sodass $f(x) - f(a) = \sum_{i = 1}^{n} q_i(x) (x - a )$.
	\end{theorem}
\end{flashcard}
\end{zettel}
\end{document}

