%! TeX root = zettel.tex
\documentclass[class=article, crop=false]{standalone}
\usepackage[subpreambles=true]{standalone}
\input{../standalone_preamble.tex}

\begin{document}
\begin{flashcard}[3nc8bvje]{Bilinearform}
	\begin{definition}
		$s: V \times  V \to K$ sd f"ur $v,w \in  V, \lambda \in  K$
		\begin{enumerate}
			\item $s (v + \lambda v', w) = s (v,w ) + \lambda s ( v;, w)$
			\item $s( v, w + \lambda w') = s (v,w) + \lambda s(v,w')$
		\end{enumerate}
	\end{definition}
\end{flashcard}

\begin{flashcard}[topmyanh]{symmetrische Bilinearform}
	\begin{definition}[symmetrische Bilinearform]
		\[
			s (v,w) = -s (w,v) \iff  s\tx{symmetrisch}
		.\]
	\end{definition}
\end{flashcard}

\begin{flashcard}[roj4sj5f]{alternierende/schiefsymmetrische Bilinearform}
	\[
		s (v,w ) = - s (w,v) \iff s \tx{alternierend/schiefsymmetrisch}
	.\]
\end{flashcard}

\begin{flashcard}[2knb18ae]{Definition $\Bil(V)$ }
	\begin{definition}
		\[
			\Bil_K(V) := \set{s: V \times  V \to  K}{\tx{Bilinearform} }
		.\]
	\end{definition}
\end{flashcard}

\begin{lemma}
	$A$ , $B \in  \Mat(n \times n; \K)$ und $s_A : K^n \times K^n \to K , \quad (x,y) \mapsto x^t \cdot A \cdot  y$ - ( ist immer bilinear)\\

	$s_B$ analog.
	\[
		s_A = s_B \iff  A = B
	.\]

\end{lemma}

\begin{theorem}
	$\Bil_K(V) \to  \Mat(n \times n; \K), s \mapsto M_{\mathcal B}(v)$ ist bijektiv. Und
	\[
		s \tx{symmetrisch (alternierend)}  \iff M_{\mathcal B } \tx{symmetrisch (alternierend)}
	.\]

\end{theorem}

\end{document}

