%! TeX root = zettel.tex
\documentclass[class=article, crop=false]{standalone}
\usepackage[subpreambles=true]{standalone}
\input{../standalone_preamble.tex}

\begin{document}
\begin{zettel}{Additivitaet}

\begin{flashcard}[jlfedjrp]{Additivitaet}
	\begin{definition}
		$R$ - Ring (oder Algebra). Dann ist $\lambda : R \to  \hat{\R }$ (mit $\exists A \in R : \lambda(A) < \infty$ ) additiv falls
		\[
			\forall A,B \in R \tx{mit} A \cap  B = \emptyset  : \lambda(A \sqcup B) = \lambda(A) + \lambda(B)
		.\]
	\end{definition}
\end{flashcard}

\begin{flashcard}[dywlxykg]{$\sigma$-Additivitaet}
	Sei $R^{\sigma}$ - $\sigma$-Ring (oder -Algebra). Dann ist $\lambda : R^\sigma \to  \hat{\R }$ (mit $\exists A \in R^\sigma : \lambda(A) < \infty$ ) $\sigma$-additiv falls
	\[
		\forall \set{A_i}_{i \in \N } \tx{mit} A_i \cap  A_j = \emptyset  \forall i \neq  j : \lambda \left( \bigsqcup_i^{\infty}A_i \right) = \sum_{i}^{\infty} \lambda(A_i)
	.\]
\end{flashcard}

\begin{flashcard}[dywlxykg]{$\sigma$-Subadditivitaet}
	Sei $R^{\sigma}$ - $\sigma$-Ring (oder -Algebra). Dann ist $\lambda : R^\sigma \to  \hat{\R }$ (mit $\exists A \in R^\sigma : \lambda(A) < \infty$ ) $\sigma$-subadditiv falls
	\[
		\forall \set{A_i}_{i \in \N } \tx{mit} A_i \cap  A_j = \emptyset  \forall i \neq  j : \lambda \left( \bigsqcup_i^{\infty}A_i \right) \leq \sum_{i}^{\infty} \lambda(A_i)
	.\]
\end{flashcard}

\begin{flashcard}[dywlxykg]{monoton (Ring, Algebra)}
	Sei $R$ -Ring (oder Algebra). Dann ist $\lambda : R \to  \hat{\R }$ (mit $\exists A \in R^\sigma : \lambda(A) < \infty$ ) monoton falls
	\[
		\forall A \in R : \lambda(A) \geq 0
	.\]
\end{flashcard}

\end{zettel}
\end{document}

